SetCover.dfy
@@ -1,20 +1,13 @@
 include "Problems.dfy"
-//include "Types.dfy"
 
 abstract module SetCoverMod{
   import opened Problems
+  import opened Auxiliary
   import opened TypeMod
 
 ghost function maximumSizeElements<T>(S:set<set<T>>):nat
 ensures forall s | s in S :: maximumSizeElements(S) >= |s|
 ensures exists s :: s in S && maximumSizeElements(S) == |s|
-
-lemma mult_preserves_order(a:int, b:int, a':int, b':int)
-  requires 0 <= a <= a'
-  requires 0 <= b <= b'
-  ensures a*b <= a'*b'
-{
-}
 
 
 
@@ -102,6 +95,9 @@ ensures counter <= counter_in + 2 + U.Size() + |U.Model()|*(U.Size() + |S.Model(
       assert counter <= counter_start_inner_loop + i*(increment_per_iteration_inner);
       assert increment_per_iteration_outer == U.Size() + |S.Model()|*(S.maximumSizeElements() + S.Size() + S.maximumSizeElements() + 1) + 3;
     }
+    else {
+      assert counter <= counter_start_inner_loop + i*(increment_per_iteration_inner);
+    }
     while !empty && !found
       decreases (if !empty && !found then 1 else 0)+|S'.Model()|
       invariant empty == (S'.Model() == {}) 
@@ -112,6 +108,7 @@ ensures counter <= counter_in + 2 + U.Size() + |U.Model()|*(U.Size() + |S.Model(
       
       invariant i == (|S.Model()| - |S'.Model()|)
       invariant counter <= counter_start_inner_loop + i*(increment_per_iteration_inner)    // *(|S.Model()| - |S'.Model()|)
+      invariant increment_per_iteration_inner == S.maximumSizeElements() + S.Size() + S.maximumSizeElements() + 1
 
       invariant increment_per_iteration_outer == U.Size() + |S.Model()|*(S.maximumSizeElements() + S.Size() + S.maximumSizeElements() + 1) + 3
     {
@@ -164,7 +161,6 @@ ensures counter <= counter_in + 2 + U.Size() + |U.Model()|*(U.Size() + |S.Model(
    
     }
     assert counter <= counter_start_inner_loop + i*(increment_per_iteration_inner);
-    assume false;
     assert i <= |S.Model()|;
     mult_preserves_order(i, increment_per_iteration_inner, |S.Model()|, increment_per_iteration_inner);
     assert counter_start_inner_loop <= counter_outer + 1 + U.Size() + 1;
@@ -197,6 +193,13 @@ ensures counter <= counter_in + 2 + U.Size() + |U.Model()|*(U.Size() + |S.Model(
   assert counter <= counter_in + 2 + U.Size() + |U.Model()|*(U.Size() + |S.Model()|*(S.maximumSizeElements() + S.Size() + S.maximumSizeElements() + 1) + 3);
   assert emptyU && b ==> U.Model()-U'.Model() == U.Model() && isCover(U.Model(),S.Model());
 
+
+  assert (emptyU && b) == isCover(U.Model(),S.Model());
+  assert size == |S.Model()|;
+  assert ((emptyU && b) && size <= k) == (isCover(U.Model(),S.Model()) &&  size <= k);
+  assert (size <= k) == (|S.Model()| <= k);
+  assert ((emptyU && b) && size <= k) == (isCover(U.Model(),S.Model()) &&  |S.Model()| <= k);
+
   b := emptyU && b && size <= k;
   assert b == (isCover(U.Model(),S.Model()) &&  |S.Model()| <= k);
   //assert counter <= counter_in + 2 + U.Size() + |U.Model()|*(U.Size() + |S.Model()|*(S.maximumSizeElements() + S.Size() + S.maximumSizeElements() + 1) + 3);
@@ -212,7 +215,83 @@ ensures counter <= counter_in + 2 + U.Size() + |U.Model()|*(U.Size() + |S.Model(
   //assert counter <= counter_in + 2 + |U.Model()|*U.Size() + |U.Model()|*|S.Model()|*S.maximumSizeElements() + |U.Model()|*|S.Model()|*S.Size() + |U.Model()|*|S.Model()|*S.maximumSizeElements() + |U.Model()|*|S.Model()|*1 + |U.Model()|*3;
 }
 
+/*
+method inner_loop<T>(empty:bool, U':Set, S':SetSet, oldU':Set, U:Set, S:SetSet, found:bool, i:int, counter_start_inner_loop:int, increment_per_iteration_inner:int, increment_per_iteration_outer:int, ghost counter_in:nat)
 
+  requires empty == (S'.Model() == {})
+  requires U'.Model() == oldU'.Model()-{e}
+  requires S'.Model()<= S.Model()
+  requires !found ==> (forall s| s in S.Model()-S'.Model():: e !in s)
+  requires found ==> exists s:set<T> :: s in S.Model() && e in s
+  requires i == (|S.Model()| - |S'.Model()|)
+  requires counter <= counter_start_inner_loop + i*(increment_per_iteration_inner)
+  requires increment_per_iteration_outer == U.Size() + |S.Model()|*(S.maximumSizeElements() + S.Size() + S.maximumSizeElements() + 1) + 3
+{
+    while !empty && !found
+      decreases (if !empty && !found then 1 else 0)+|S'.Model()|
+      invariant empty == (S'.Model() == {}) 
+      invariant U'.Model() == oldU'.Model()-{e}
+      invariant S'.Model()<= S.Model()
+      invariant !found ==> (forall s| s in S.Model()-S'.Model():: e !in s)
+      invariant found ==> exists s:set<T> :: s in S.Model() && e in s
+      
+      invariant i == (|S.Model()| - |S'.Model()|)
+      invariant counter <= counter_start_inner_loop + i*(increment_per_iteration_inner)    // *(|S.Model()| - |S'.Model()|)
+      invariant increment_per_iteration_inner == S.maximumSizeElements() + S.Size() + S.maximumSizeElements() + 1
+
+      invariant increment_per_iteration_outer == U.Size() + |S.Model()|*(S.maximumSizeElements() + S.Size() + S.maximumSizeElements() + 1) + 3
+    {
+     ghost var counter_inner := counter;
+     assert counter_inner <= counter_start_inner_loop + i*(increment_per_iteration_inner);
+     ghost var prev_i := i;
+    
+     assert S'.maximumSizeElements() <= S.maximumSizeElements();
+  
+     var s;
+     ghost var oldS':= S';
+     s,counter := S'.Pick(counter); //+maxS
+     assert |oldS'.Model()| == |S'.Model()|;
+     assert oldS' == S';
+     
+     ghost var counter_1 := counter;
+     assert s.Model() in S'.Model();
+     S',counter := S'.Remove(s,counter);//+|S|*maxS
+     assert |S'.Model()| == |oldS'.Model()| - 1;
+     
+     assert counter == counter_1 + oldS'.Size();
+     assert counter_1 == counter_inner + oldS'.maximumSizeElements();
+     assert counter == counter_inner + oldS'.maximumSizeElements() + oldS'.Size();
+     
+     ghost var counter_2 := counter;
+     found,counter := s.Contains(e,counter);//+maxS*sizeT
+     empty,counter := S'.Empty(counter);//+1
+     assert counter <= counter_2 + S.maximumSizeElements() + 1;
+              //Total suma <= maxS*(|S| + sizeT + 1)+1
+     
+     assert counter <= counter_inner + oldS'.maximumSizeElements() + oldS'.Size() + S.maximumSizeElements() + 1;
+     assert 0 <= |oldS'.Model()| <= |S.Model()|;
+     assert 0 <= oldS'.maximumSizeElements() <= S.maximumSizeElements();
+    
+     mult_preserves_order(|oldS'.Model()|, oldS'.maximumSizeElements(), |S.Model()|, S.maximumSizeElements());
+     assert |oldS'.Model()|*oldS'.maximumSizeElements() <= |S.Model()|*S.maximumSizeElements();
+
+     assert oldS'.Size() == |oldS'.Model()|*oldS'.maximumSizeElements();
+     assert S.Size() == |S.Model()|*S.maximumSizeElements();
+
+     assert oldS'.Size() <= S.Size();
+     assert counter <= counter_inner + S.maximumSizeElements() + S.Size() + S.maximumSizeElements() + 1;
+     assert counter_inner <= counter_start_inner_loop + i*(increment_per_iteration_inner);
+     
+     i := i + 1;
+     assert i == prev_i + 1;
+     assert counter <= counter_inner + increment_per_iteration_inner;
+     assert counter_inner <= counter_start_inner_loop + (i-1)*(increment_per_iteration_inner);
+     assert counter <= counter_start_inner_loop + i*(increment_per_iteration_inner);
+   
+    }
+}
+
+*/
 
 
 
